src/coq/Handlers/Concretization.v
@@ -1002,9 +1002,6 @@ Module MakeBase (LP : LLVMParams) (MP : MemoryParams LP) (Byte : ByteModule LP.A
   Section Concretize.
 
 
-
-    Variable endianess : Endianess.
-
     (* Convert a list of UVALUE_ExtractByte values into a dvalue of
          a given type.
 
@@ -1410,6 +1407,105 @@ Module MakeBase (LP : LLVMParams) (MP : MemoryParams LP) (Byte : ByteModule LP.A
       unfold list_sum.
       lia.
     Qed.
+
+    Lemma dvalue_bytes_to_dvalue_equation
+      {M} `{HM : Monad M} `{RE: RAISE_ERROR M} `{RP: RAISE_POISON M} `{RO: RAISE_OOMABLE M} (dbs : list dvalue_byte) (dt : dtyp) :
+      @dvalue_bytes_to_dvalue M HM RE RP RO dbs dt =
+        match dt with
+        | DTYPE_I sz =>
+            zs <- map_monad dvalue_byte_value dbs;;
+            match sz with
+            | 1 =>
+                ret (DVALUE_I1 (concat_bytes_Z_vint zs))
+            | 8 =>
+                ret (DVALUE_I8 (concat_bytes_Z_vint zs))
+            | 32 =>
+                ret (DVALUE_I32 (concat_bytes_Z_vint zs))
+            | 64 =>
+                ret (DVALUE_I64 (concat_bytes_Z_vint zs))
+            | _ => raise_error "Unsupported integer size."
+            end
+        | DTYPE_IPTR =>
+            zs <- map_monad dvalue_byte_value dbs;;
+            val <- lift_OOMABLE DTYPE_IPTR (IP.from_Z (concat_bytes_Z zs));;
+            ret (DVALUE_IPTR val)
+        | DTYPE_Pointer =>
+            (* TODO: not sure if this should be wildcard provenance.
+                TODO: not sure if this should truncate iptr value...
+             *)
+            (* TODO: not sure if this should be lazy OOM or not *)
+            zs <- map_monad dvalue_byte_value dbs;;
+            match int_to_ptr (concat_bytes_Z zs) wildcard_prov with
+            | NoOom a => ret (DVALUE_Addr a)
+            | Oom msg => raise_oomable DTYPE_Pointer
+            end
+        | DTYPE_Void =>
+            raise_error "dvalue_bytes_to_dvalue on void type."
+        | DTYPE_Half =>
+            raise_error "dvalue_bytes_to_dvalue: unsupported DTYPE_Half."
+        | DTYPE_Float =>
+            zs <- map_monad dvalue_byte_value dbs;;
+            ret (DVALUE_Float (Float32.of_bits (concat_bytes_Z_vint zs)))
+        | DTYPE_Double =>
+            zs <- map_monad dvalue_byte_value dbs;;
+            ret (DVALUE_Double (Float.of_bits (concat_bytes_Z_vint zs)))
+        | DTYPE_X86_fp80 =>
+            raise_error "dvalue_bytes_to_dvalue: unsupported DTYPE_X86_fp80."
+        | DTYPE_Fp128 =>
+            raise_error "dvalue_bytes_to_dvalue: unsupported DTYPE_Fp128."
+        | DTYPE_Ppc_fp128 =>
+            raise_error "dvalue_bytes_to_dvalue: unsupported DTYPE_Ppc_fp128."
+        | DTYPE_Metadata =>
+            raise_error "dvalue_bytes_to_dvalue: unsupported DTYPE_Metadata."
+        | DTYPE_X86_mmx =>
+            raise_error "dvalue_bytes_to_dvalue: unsupported DTYPE_X86_mmx."
+        | DTYPE_Array sz t =>
+            let sz := sizeof_dtyp t in
+            elt_bytes <- lift_err_RAISE_ERROR (split_every sz dbs);;
+            elts <- map_monad (fun es => dvalue_bytes_to_dvalue es t) elt_bytes;;
+            ret (DVALUE_Array elts)
+        | DTYPE_Vector sz t =>
+            let sz := sizeof_dtyp t in
+            elt_bytes <- lift_err_RAISE_ERROR (split_every sz dbs);;
+            elts <- map_monad (fun es => dvalue_bytes_to_dvalue es t) elt_bytes;;
+            ret (DVALUE_Vector elts)
+        | DTYPE_Struct fields =>
+            match fields with
+            | [] => ret (DVALUE_Struct []) (* TODO: Not 100% sure about this. *)
+            | (dt::dts) =>
+                let sz := sizeof_dtyp dt in
+                let init_bytes := take sz dbs in
+                let rest_bytes := drop sz dbs in
+                f <- dvalue_bytes_to_dvalue init_bytes dt;;
+                rest <- dvalue_bytes_to_dvalue rest_bytes (DTYPE_Struct dts);;
+                match rest with
+                | DVALUE_Struct fs =>
+                    ret (DVALUE_Struct (f::fs))
+                | _ =>
+                    raise_error "dvalue_bytes_to_dvalue: DTYPE_Struct recursive call did not return a struct."
+                end
+            end
+        | DTYPE_Packed_struct fields =>
+            match fields with
+            | [] => ret (DVALUE_Packed_struct []) (* TODO: Not 100% sure about this. *)
+            | (dt::dts) =>
+                let sz := sizeof_dtyp dt in
+                let init_bytes := take sz dbs in
+                let rest_bytes := drop sz dbs in
+                f <- dvalue_bytes_to_dvalue init_bytes dt;;
+                rest <- dvalue_bytes_to_dvalue rest_bytes (DTYPE_Struct dts);;
+                match rest with
+                | DVALUE_Packed_struct fs =>
+                    ret (DVALUE_Packed_struct (f::fs))
+                | _ =>
+                    raise_error "dvalue_bytes_to_dvalue: DTYPE_Packed_struct recursive call did not return a struct."
+                end
+            end
+        | DTYPE_Opaque =>
+            raise_error "dvalue_bytes_to_dvalue: unsupported DTYPE_Opaque."
+        end.
+    Proof.
+    Admitted.
 
     Definition uvalue_sid_match (a b : uvalue) : bool
       :=
@@ -1819,6 +1915,71 @@ Module MakeBase (LP : LLVMParams) (MP : MemoryParams LP) (Byte : ByteModule LP.A
         intros u.
         unfold concretize_uvalueM at 1.
         destruct u; try reflexivity.
+      Qed.
+
+      Lemma extractbytes_to_dvalue_equation :
+        forall uvs dt,
+          extractbytes_to_dvalue uvs dt =
+            dvbs <- concretize_uvalue_bytes uvs;;
+            lift_ue (ErrOOMPoison_handle_poison_and_oom_dv (dvalue_bytes_to_dvalue dvbs dt)).
+      Proof.
+        induction uvs;
+          intros dt;
+          unfold extractbytes_to_dvalue.
+        - Opaque ErrOOMPoison_handle_poison_and_oom_dv
+            dvalue_bytes_to_dvalue.
+          cbn.
+          reflexivity.
+        - destruct a;
+            cbn; auto.
+      Qed.
+
+      Lemma concretize_uvalue_bytes_helper_equation :
+        forall acc uvs,
+          concretize_uvalue_bytes_helper acc uvs =
+            match uvs with
+            | [] => ret []
+            | (uv::uvs) =>
+                match uv with
+                | UVALUE_ExtractByte byte_uv dt idx sid =>
+                    (* Check if this uvalue has been concretized already *)
+                    match pre_concretized acc byte_uv sid with
+                    | Some dv =>
+                        (* Use the pre_concretized value *)
+                        let dv_byte := DVALUE_ExtractByte dv dt idx in
+                        (* Concretize the rest of the bytes *)
+                        rest <- concretize_uvalue_bytes_helper acc uvs;;
+                        ret (dv_byte :: rest)
+                    | None =>
+                        (* Concretize the uvalue *)
+                        dv <- concretize_uvalueM byte_uv;;
+                        let dv_byte := DVALUE_ExtractByte dv dt idx in
+                        let acc := new_concretized_byte acc byte_uv dv sid in
+                        (* Concretize the rest of the bytes *)
+                        rest <- concretize_uvalue_bytes_helper acc uvs;;
+                        ret (dv_byte :: rest)
+                    end
+                | _ =>
+                    lift_ue (raise_error "concretize_uvalue_bytes_helper: non-byte in uvs.")
+                end
+            end.
+      Proof.
+        intros acc uvs;
+          induction uvs;
+          unfold concretize_uvalue_bytes_helper.
+        - reflexivity.
+        - destruct a;
+            reflexivity.
+      Qed.
+
+      Lemma concretize_uvalue_bytes_equation (uvs : list uvalue) :
+        concretize_uvalue_bytes uvs =
+          concretize_uvalue_bytes_helper (@NM.empty _) uvs.
+      Proof.
+        induction uvs;
+          unfold concretize_uvalue_bytes.
+        - reflexivity.
+        - destruct a; reflexivity.
       Qed.
 
       Lemma eval_select_equation :
